books/evm/exec-defthms.lisp
@@ -7,28 +7,30 @@
 (include-book "exec")
 (include-book "op-exec-defthms")
 
-(defthm env/step-io-pc-validp
-    (implies (env/validp e)
-             (integerp (env/pc (env/step e)))))
-
 ;; The proof checking takes about 10 minutes.
 (defthm env/step-io-validp
     (implies (env/validp e)
-             (env/validp (env/step e))))
+             (env/validp (env/step e)))
+  :hints (("Goal" :in-theory (enable env/step))))
+
+;; (defthm env/exec-hacky-io-validp
+;;     (implies (env/validp e)
+;;              (env/validp (env/exec-hacky e n))))
+
+;; (defthm env/exec-valid-io
+;;     (implies (env/validp e)
+;;              (env/validp (env/exec e))))
+
+;; ---- Just some experiments ----
+
+;; (defthm env/step-io-pc-validp
+;;     (implies (env/validp e)
+;;              (integerp (env/pc (env/step e))))
+;;   :hints (("Goal" :in-theory (enable env/step))))
+
 
 ;; The proof checking takes 12000+ seconds.
 ;; (defthm env/exec-hacky-io-pc-validp
 ;;     (implies (env/validp e)
 ;;              (integerp (env/pc (env/exec-hacky e n))))
-;;   :hints (("Goal" :in-theory (disable stack/pop
-;;                                       stack/push))))
-
-;; (defthm env/exec-hacky-io-validp
-;;     (implies (env/validp e)
-;;              (env/validp (env/exec-hacky e n)))
-;;   :hints (("Goal" :in-theory (disable stack/pop
-;;                                       stack/push))))
-
-;; (defthm env/exec-valid-io
-;;     (implies (env/validp e)
-;;              (env/validp (env/exec e))))
+;;   :hints (("Goal" :in-theory (disable env/step))))
